Update file2.dfy

file2.dfy
@@ -22,18 +22,29 @@ predicate isOptSol(sol : seq<int>, nr:int)
     requires sol[0]>=0
     requires sol[1]>=0
     requires sol[2]>=0
-    requires isSol(sol,nr)
 {   
-
+  isSol(sol,nr) &&
   forall sol' :: |sol'| == 3 && sol'[0]>=0 && sol'[1]>=0 && sol'[2]>=0 && isSol(sol',nr) ==> cost(sol') >= cost(sol)
 
 }
 
+predicate INV(copie: int, nr: int, s1: int, s5: int, s10:int)
+  requires s1 >= 0
+  requires s5 >= 0
+  requires s10 >= 0
+{
+   forall s1', s5', s10' :: s1'>=0 && s5'>=0 && s10'>=0 
+          && isOptSol([s1',s5',s10'],copie) ==> 
+          isOptSol([s1+s1',s5+s5',s10+s10'],nr)
+}
 
 
 method findMax(nr: int) returns(s:int)
-    requires nr != 0
-    ensures s>0
+  requires nr>0
+    ensures 0<s <= nr
+    ensures s == 1 || s==5 || s==10
+    ensures s==1 ==> nr< 5
+  
 {
   var a := new int[3];
   a[0], a[1], a[2] := 1, 5, 10;
@@ -42,7 +53,8 @@ method findMax(nr: int) returns(s:int)
   //3 if 
   while (i<a.Length && a[i] <= nr)
     invariant 0 <= i <= a.Length
-    invariant s>0
+    invariant 0<s<=nr
+    invariant s == 1 || s==5 || s==10
   {
     s := a[i];
     i := i + 1;
@@ -50,39 +62,86 @@ method findMax(nr: int) returns(s:int)
 }
 
 
+lemma caz1(copie: int, nr: int, s1: int, s5: int, s10: int)
+  requires copie < 5
+  requires s1 >= 0
+  requires s5 >= 0
+  requires s10 >= 0
+  requires INV(copie,nr,s1,s5,s10)
+  ensures INV(copie-1,nr,s1+1,s5,s10)
+{
+  assume false;
+}
+
+lemma caz2(copie: int,nr: int,s1: int,s5: int,s10: int)
+  requires copie >= 5
+  requires s1 >= 0
+  requires s5 >= 0
+  requires s10 >= 0
+  requires INV(copie,nr,s1,s5,s10)
+  ensures INV(copie-5,nr,s1,s5+1,s10)
+{
+  assume false;
+}
+
+lemma caz3(copie: int,nr: int,s1: int,s5: int,s10: int)
+  requires copie >= 10
+  requires s1 >= 0
+  requires s5 >= 0
+  requires s10 >= 0
+  requires INV(copie,nr,s1,s5,s10)
+  ensures INV(copie-10,nr,s1,s5,s10+1)
+{
+  assume false;
+}
+
+
   method bancnote(nr: int) returns (sol: seq<int>)
-    requires nr != 0
+    requires nr>=0
     ensures |sol| == 3
-    requires sol[0]>=0
-    requires sol[1]>=0
-    requires sol[2]>=0
+    ensures sol[0]>=0
+    ensures sol[1]>=0
+    ensures sol[2]>=0
+    ensures isSol(sol,nr)
     ensures isOptSol(sol,nr)
-  {
+{
     var copie:=  nr;
     var s1 := 0;
     var s5 := 0;
     var s10 := 0;
     while(copie > 0)
       decreases copie
+      invariant 0<=copie<=nr
+      invariant isSol([s1,s5,s10],nr-copie)
+      invariant INV(copie,nr,s1,s5,s10)
     {
         var i := 0;
         var s := findMax(copie);
         if( s == 1){
+          caz1(copie,nr,s1,s5,s10);
             s1:=s1+1;
+            assert isSol([s1,s5,s10],nr-(copie-1));
+            assert INV(copie-1,nr,s1,s5,s10);
         }
         else{
             if(s == 5)
             {
                 s5:=s5+1;
+                assert isSol([s1,s5,s10],nr-(copie-5));
+              
+                assert INV(copie-5,nr,s1,s5,s10);
+
             }
             else{
                 s10:=s10+1;
+                assert isSol([s1,s5,s10],nr-(copie-10));
+                assert INV(copie-10,nr,s1,s5,s10);
+
             }
         }
         copie := copie-s;
     }
     sol := [s1,s5,s10];
-
 
   }
 
